@prefix rdf: <http://www.w3.org/1999/02/22-rdf-syntax-ns#> .
@prefix : <http://linda-project.eu/linda-visualization#> .
@prefix common: <http://linda-project.eu/common#> .
@prefix terms: <http://purl.org/dc/terms/> .
@prefix owl: <http://www.w3.org/2002/07/owl#> .
@prefix xsd: <http://www.w3.org/2001/XMLSchema#> .
@prefix rdfs: <http://www.w3.org/2000/01/rdf-schema#> .

<http://linda-project.eu/linda-visualization#>
    a owl:Ontology ;
    rdfs:comment "LinDA Visualization Vocabulary"@de ;
    owl:versionInfo "0.1" .

:AreaChart
    :layoutOption [
        :optionName "Horizontal Label" ;
        :optionType xsd:string ;
        :optionValue "Label"^^xsd:string ;
        a :Option
    ], [
        :optionName "Vertical Label" ;
        :optionType xsd:string ;
        :optionValue "Label"^^xsd:string ;
        a :Option
    ], [
        :optionName "Gridlines" ;
        :optionType xsd:nonNegativeInteger ;
        :optionValue "10"^^xsd:nonNegativeInteger ;
        a :Option
    ], [
        :optionName "Tooltip" ;
        :optionType xsd:boolean ;
        :optionValue "true"^^xsd:boolean ;
        a :Option
    ] ;
    :structureOption [
        :optionName "Horizontal Axis" ;
        :optionType [
            :maxCardinality "1"^^xsd:nonNegativeInteger ;
            :minCardinality "1"^^xsd:nonNegativeInteger ;
            :scaleOfMeasurement :Interval ;
            :dimensionRole :Domain ;
            a :Dimension
        ] ;
        a :Option
    ], [
        :optionName "Vertical Axis" ;
        :optionType [
            :maxCardinality "1"^^xsd:nonNegativeInteger ;
            :minCardinality "1"^^xsd:nonNegativeInteger ;
            :scaleOfMeasurement :Ratio ;
            :dimensionRole :Range ;
            a :Dimension
        ] ;
        a :Option
    ], [
        :optionName "Series" ;
        :optionType [
            :maxCardinality "1"^^xsd:nonNegativeInteger ;
            :scaleOfMeasurement :Nominal ;
            :dimensionRole :Domain ;
            a :Dimension
        ] ;
        a :Option
    ] ;
    :visualizationType :PartToWhole, :TimeSeries ;
    :visualizationName "AreaChart" ;

    a :Visualization, owl:NamedIndividual ;
    rdfs:comment "An area chart is a variation of line chart and shows a filled area below the quantity line. It is used to visualize part-to-whole relationships between several time series and their cumulative values."@en .

:BarChart
    :layoutOption [
        :optionName "Horizontal Label" ;
        :optionType xsd:string ;
        :optionValue "Label"^^xsd:string ;
        a :Option
    ], [
        :optionName "Vertical Label" ;
        :optionType xsd:string ;
        :optionValue "Label"^^xsd:string ;
        a :Option
    ], [
        :optionName "Gridlines" ;
        :optionType xsd:nonNegativeInteger ;
        :optionValue "10"^^xsd:nonNegativeInteger ;
        a :Option
    ], [
        :optionName "Tooltip" ;
        :optionType xsd:boolean ;
        :optionValue "true"^^xsd:boolean ;
        a :Option
    ] ;
    :structureOption [
        :optionName "Horizontal Axis" ;
        :optionType [
            :maxCardinality "1"^^xsd:nonNegativeInteger ;
            :minCardinality "1"^^xsd:nonNegativeInteger ;
            :scaleOfMeasurement :Nominal ;
            :dimensionRole :Domain ;
            a :Dimension
        ] ;
        a :Option
    ], [
        :optionName "Vertical Axis" ;
        :optionType [
            :maxCardinality "1"^^xsd:nonNegativeInteger ;
            :minCardinality "1"^^xsd:nonNegativeInteger ;
            :scaleOfMeasurement :Interval, :Ratio ;
            :dimensionRole :Range ;
            a :Dimension
        ] ;
        a :Option
    ], [
        :optionName "Groups" ;
        :optionType [
            :maxCardinality "1"^^xsd:nonNegativeInteger ;
            :scaleOfMeasurement :Nominal ;
            :dimensionRole :Domain ;
            a :Dimension
        ] ;
        a :Option
    ] ;
    :visualizationType :Comparison, :PartToWhole, :TimeSeries ;
    :visualizationName "BarChart" ;
    a :Visualization, owl:NamedIndividual ;
    rdfs:comment "A graph used to display and compare the number, frequency or other measure for different discrete categories of data."@en .

:BubbleChart
    :layoutOption [
        :optionName "Horizontal Label" ;
        :optionType xsd:string ;
        :optionValue "Label"^^xsd:string ;
        a :Option
    ], [
        :optionName "Vertical Label" ;
        :optionType xsd:string ;
        :optionValue "Label"^^xsd:string ;
        a :Option
    ], [
        :optionName "Gridlines" ;
        :optionType xsd:nonNegativeInteger ;
        :optionValue "10"^^xsd:nonNegativeInteger ;
        a :Option
    ], [
        :optionName "Tooltip" ;
        :optionType xsd:boolean ;
        :optionValue "true"^^xsd:boolean ;
        a :Option
    ] ;
    :structureOption [
        :optionName "Horizontal Axis" ;
        :optionType [
            :maxCardinality "1"^^xsd:nonNegativeInteger ;
            :minCardinality "1"^^xsd:nonNegativeInteger ;
            :scaleOfMeasurement :Interval, :Ratio ;
            :dimensionRole :Range ;
            a :Dimension
        ] ;
        a :Option
    ], [
        :optionName "Vertical Axis" ;
        :optionType [
            :maxCardinality "1"^^xsd:nonNegativeInteger ;
            :minCardinality "1"^^xsd:nonNegativeInteger ;
            :scaleOfMeasurement :Interval, :Ratio ;
            :dimensionRole :Range ;
            a :Dimension
        ] ;
        a :Option
    ], [
        :optionName "Size" ;
        :optionType [
            :maxCardinality "1"^^xsd:nonNegativeInteger ;
            :minCardinality "1"^^xsd:nonNegativeInteger ;
            :scaleOfMeasurement :Ratio ;
            :dimensionRole :Range ;
            a :Dimension
        ] ;
        a :Option
    ], [
        :optionName "Groups" ;
        :optionType [
            :maxCardinality "1"^^xsd:nonNegativeInteger ;
            :scaleOfMeasurement :Nominal ;
            a :Dimension
        ] ;
        a :Option
    ], [
        :optionName "Label" ;
        :optionType [
            :maxCardinality "1"^^xsd:nonNegativeInteger ;
            :scaleOfMeasurement :Nominal ;
            :dimensionRole :Domain ;
            a :Dimension
        ] ;
        a :Option
    ] ;
    :visualizationType :Comparison, :Correlation ;
    :visualizationName "BubbleChart" ;
    a :Visualization, owl:NamedIndividual ;
    rdfs:comment "A graph is used to display three dimensional data, where the third dimension is a size of a bubble. The fourth dimension could be embedded as a color of bubbles."@en .

:Comparison
    a :TypeOfVisualization, owl:NamedIndividual ;
    rdfs:comment "Type of visualization"@en ;
    rdfs:label "Comparison"@en .

:Correlation
    a :TypeOfVisualization, owl:NamedIndividual ;
    rdfs:comment "Type of visualization"@en ;
    rdfs:label "Correlation"@en .

:Dimension
    a owl:Class ;
    rdfs:comment "The type of structure options"@en ;
    rdfs:label "Dimension"@en .

:Distribution
    a :TypeOfVisualization, owl:NamedIndividual ;
    rdfs:comment "Type of visualization"@en ;
    rdfs:label "Distribution"@en .

:Geographical
    a :TypeOfVisualization, owl:NamedIndividual ;
    rdfs:comment "Type of visualization"@en ;
    rdfs:label "Geographical"@en .

:LineChart
    :layoutOption [
        :optionName "Horizontal Label" ;
        :optionType xsd:string ;
        :optionValue "Label"^^xsd:string ;
        a :Option
    ], [
        :optionName "Vertical Label" ;
        :optionType xsd:string ;
        :optionValue "Label"^^xsd:string ;
        a :Option
    ], [
        :optionName "Gridlines" ;
        :optionType xsd:nonNegativeInteger ;
        :optionValue "10"^^xsd:nonNegativeInteger ;
        a :Option
    ], [
        :optionName "Tooltip" ;
        :optionType xsd:boolean ;
        :optionValue "true"^^xsd:boolean ;
        a :Option
    ] ;
    :structureOption [
        :optionName "Horizontal Axis" ;
        :optionType [
            :maxCardinality "1"^^xsd:nonNegativeInteger ;
            :minCardinality "1"^^xsd:nonNegativeInteger ;
            :scaleOfMeasurement :Interval ;
            :dimensionRole :Domain ;
            a :Dimension
        ] ;
        a :Option
    ], [
        :optionName "Vertical Axis" ;
        :optionType [
            :maxCardinality "1"^^xsd:nonNegativeInteger ;
            :minCardinality "1"^^xsd:nonNegativeInteger ;
            :scaleOfMeasurement :Interval, :Ratio ;
            :dimensionRole :Range ;
            a :Dimension
        ] ;
        a :Option
    ], [
        :optionName "Series" ;
        :optionType [
            :maxCardinality "1"^^xsd:nonNegativeInteger ;
            :scaleOfMeasurement :Nominal ;
            :dimensionRole :Domain ;
            a :Dimension
        ] ;
        a :Option
    ] ;
    :visualizationType :TimeSeries ;
    :visualizationName "LineChart" ;
    a :Visualization, owl:NamedIndividual ;
    rdfs:comment "A graph used to visualize a trend in data over intervals of time. Line charts emphasize time flow and rate of change rather than the amount of change."@en .

:Map
    :structureOption [
        :optionName "Latitude" ;
        :optionType [
            :maxCardinality "1"^^xsd:nonNegativeInteger ;
            :minCardinality "1"^^xsd:nonNegativeInteger ;
            :scaleOfMeasurement :GeographicLatitude ;
            :associatedProperty <http://www.w3.org/2003/01/geo/wgs84_pos#lat> ;
            a :Dimension
        ] ;
        a :Option
    ], [
        :optionName "Longitude" ;
        :optionType [
            :maxCardinality "1"^^xsd:nonNegativeInteger ;
            :minCardinality "1"^^xsd:nonNegativeInteger ;
            :scaleOfMeasurement :GeographicLongitude ;
            :associatedProperty <http://www.w3.org/2003/01/geo/wgs84_pos#long> ;
            a :Dimension
        ] ;
        a :Option
    ], [
        :optionName "Label" ;
        :optionType [
            :minCardinality "1"^^xsd:nonNegativeInteger ;
            :scaleOfMeasurement :Nominal ;
            a :Dimension
        ] ;
        a :Option
    ], [
        :optionName "Indicator" ;
        :optionType [
            :scaleOfMeasurement :Ratio ;
            :dimensionRole :Range ;
            a :Dimension
        ] ;
        a :Option
    ] ;
    :visualizationType :Comparison, :Geographical ;
    :visualizationName "Map" ;
    a :Visualization, owl:NamedIndividual ;
    rdfs:comment "A visualization used for displaying geographical data on a map."@en .


:Option
    a owl:Class ;
    rdfs:comment ""@en ;
    rdfs:label "Option"@en .


:PartToWhole
    a :TypeOfVisualization, owl:NamedIndividual ;
    rdfs:comment "Type of visualization"@en ;
    rdfs:label "Part-To-Whole"@en .

:PieChart
    :layoutOption [
        :optionName "Horizontal Label" ;
        :optionType xsd:string ;
        :optionValue "Label"^^xsd:string ;
        a :Option
    ], [
        :optionName "Vertical Label" ;
        :optionType xsd:string ;
        :optionValue "Label"^^xsd:string ;
        a :Option
    ], [
        :optionName "Tooltip" ;
        :optionType xsd:boolean ;
        :optionValue "true"^^xsd:boolean ;
        a :Option
    ] ;
    :structureOption [
        :optionName "Measure" ;
        :optionType [
            :maxCardinality "1"^^xsd:nonNegativeInteger ;
            :minCardinality "1"^^xsd:nonNegativeInteger ;
            :scaleOfMeasurement :Ratio ;
            :dimensionRole :Range ;
            a :Dimension
        ] ;
        a :Option
    ], [
        :optionName "Slices" ;
        :optionType [
            :maxCardinality "6"^^xsd:nonNegativeInteger ;
            :minCardinality "1"^^xsd:nonNegativeInteger ;
            :scaleOfMeasurement :Nominal ; 
            :dimensionRole :Domain ;
            a :Dimension
        ] ;
        a :Option
    ] ;
    :visualizationType :PartToWhole ;
    :visualizationName "PieChart" ;
    a :Visualization, owl:NamedIndividual ;
    rdfs:comment "A graph used for visualizing the relative contribution that different categories contribute to an overall total."@en .


:ScaleOfMeasurement
    a owl:Class ;
    rdfs:comment "Scale Of Measurement: Categorical (nominal, ordinal), Quantitative (Interval) data"@en ;
    rdfs:label "Scale Of Measurement"@en .

:ScaleOfMeasurementForCategoricalData
    a owl:Class ;
    rdfs:comment "Scale Of Measurement for categorical data: nominal, ordinal"@en ;
    rdfs:label "SoM Categorical Data"@en ;
    rdfs:subClassOf :ScaleOfMeasurement .

:ScaleOfMeasurementForQuantitativeData
    a owl:Class ;
    rdfs:comment "Scale Of Measurement for quantitative data: interval, ratio"@en ;
    rdfs:label "SoM Quantitative Data"@en ;
    rdfs:subClassOf :ScaleOfMeasurement .

:DimensionRole
    a owl:Class ;
    rdfs:comment "The role a dimension plays in the functional description of its visualization: Domain (called Dimension in Data Cube) or Range (Measure in Data Cube)"@en .

:ScatterChart
    :layoutOption [
        :optionName "Horizontal Label" ;
        :optionType xsd:string ;
        :optionValue "Label"^^xsd:string ;
        a :Option
    ], [
        :optionName "Vertical Label" ;
        :optionType xsd:string ;
        :optionValue "Label"^^xsd:string ;
        a :Option
    ], [
        :optionName "Gridlines" ;
        :optionType xsd:nonNegativeInteger ;
        :optionValue "10"^^xsd:nonNegativeInteger ;
        a :Option
    ], [
        :optionName "Tooltip" ;
        :optionType xsd:boolean ;
        :optionValue "true"^^xsd:boolean ;
        a :Option
    ] ;
    :structureOption [
        :optionName "Horizontal Axis" ;
        :optionType [
            :maxCardinality "1"^^xsd:nonNegativeInteger ;
            :minCardinality "1"^^xsd:nonNegativeInteger ;
            :scaleOfMeasurement :Ratio ;
            :dimensionRole :Range ;
            a :Dimension
        ] ;
        a :Option
    ], [
        :optionName "Vertical Axis" ;
        :optionType [
            :maxCardinality "1"^^xsd:nonNegativeInteger ;
            :minCardinality "1"^^xsd:nonNegativeInteger ;
            :scaleOfMeasurement :Ratio ;
            :dimensionRole :Range ;
            a :Dimension
        ] ;
        a :Option
    ], [
        :optionName "Groups" ;
        :optionType [
            :maxCardinality "1"^^xsd:nonNegativeInteger ;
            :scaleOfMeasurement :Nominal ;
            a :Dimension
        ] ;
        a :Option
    ] ;
    :visualizationType :Comparision, :Correlation ;
    :visualizationName "ScatterChart" ;
    a :Visualization, owl:NamedIndividual ;
    rdfs:comment "A graph used to show the relationship between pairs of quantitative measurements."@en .

:Domain
    a :DimensionRole, owl:NamedIndividual ;
    rdfs:comment "'Domain' dimension role, also known as 'dimension' in Data Cube, or as 'independent variable'"@en ;
    rdfs:label "Domain"@en .

:Range
    a :DimensionRole, owl:NamedIndividual ;
    rdfs:comment "'Range' dimension role, also known as 'measure' in Data Cube, or as 'dependent variable'"@en ;
    rdfs:label "Range"@en .

:TimeSeries
    a :TypeOfVisualization, owl:NamedIndividual ;
    rdfs:comment "Type of visualization"@en ;
    rdfs:label "Time Series"@en .

:TypeOfVisualization
    a owl:Class ;
    rdfs:comment "Type of visualization: Comparision, Time Series, Part-To-Whole, Distribution, Correlation"@en ;
    rdfs:label "Type Of Visualization"@en .

:Visualization
    a owl:Class ;
    rdfs:comment ""@en ;
    rdfs:label "Visualization"@en .

:VisualizationConfiguration
    a owl:Class ;
    rdfs:comment ""@en ;
    rdfs:label "Visualization Configuration"@en ;
    rdfs:subClassOf :Visualization .

:configurationName
    a owl:DatatypeProperty ;
    rdfs:comment "Visualization Configuration Name"@en ;
    rdfs:domain :VisualizationConfiguration ;
    rdfs:label "Visualization Name"@en ;
    rdfs:range xsd:string .

:configurationID
    a owl:DatatypeProperty ;
    rdfs:comment ""@en ;
    rdfs:domain :VisualizationConfiguration ;
    rdfs:label "Visualization_ID"@en ;
    rdfs:range xsd:nonNegativeInteger .

:datasource
    a owl:DatatypeProperty ;
    rdfs:comment ""@en ;
    rdfs:domain :VisualizationConfiguration ;
    rdfs:label "Visualization Configuration Datasource"@en ;
    rdfs:range xsd:anyURI .

:layoutOptions
    a owl:ObjectProperty ;
    rdfs:comment ""@en ;
    rdfs:domain :Visualization ;
    rdfs:label "Layout_Options"@en ;
    rdfs:range :Option .

:maxCardinality
    a owl:DatatypeProperty ;
    rdfs:comment "The maximum number of properties mapped to the dimension. "@en ;
    rdfs:domain :Dimension ;
    rdfs:label "Maximum cardinality"@en ;
    rdfs:range xsd:nonNegativeInteger .

:minCardinality
    a owl:DatatypeProperty ;
    rdfs:comment "The minimum number of properties mapped to the dimension. "@en ;
    rdfs:domain :Dimension ;
    rdfs:label "Minimum cardinality"@en ;
    rdfs:range xsd:nonNegativeInteger .

:optionName
    a owl:DatatypeProperty ;
    rdfs:comment ""@en ;
    rdfs:domain :Option ;
    rdfs:label "Option Name"@en ;
    rdfs:range xsd:string .

:optionType
    a owl:ObjectProperty ;
    rdfs:comment "Can be a Dimension (structure option), or xsd:string, xsd:number, xsd:boolean (layout options) "@en ;
    rdfs:domain :Option ;
    rdfs:label "Option_Type"@en .

:scaleOfMeasurement
    a owl:ObjectProperty ;
    rdfs:comment "The scale of measurement of a dimension. "@en ;
    rdfs:domain :Dimension ;
    rdfs:label "Scale of measurement"@en ;
    rdfs:range :ScaleOfMeasurement .

:dimensionRole
    a owl:ObjectProperty ;
    rdfs:comment "The role of a dimension"@en ;
    rdfs:domain :Dimension ;
    rdfs:label "Role"@en ;
    rdfs:range :DimensionRole .

:associatedProperty
    a owl:ObjectProperty ;
    rdfs:comment "An RDF property associated with a dimension, e.g. wgs84:lat for a map's latitude"@en ;
    rdfs:domain :Dimension ;
    rdfs:label "Associated property"@en ;
    rdfs:range owl:DatatypeProperty .

:structureOption
    a owl:ObjectProperty ;
    rdfs:comment ""@en ;
    rdfs:domain :Visualization ;
    rdfs:label "Structure_Option"@en ;
    rdfs:range :Option .

:visualizationName
    a owl:DatatypeProperty ;
    rdfs:comment ""@en ;
    rdfs:domain :Visualization ;
    rdfs:label "Visualization Name"@en ;
    rdfs:range xsd:string .

:moreSpecificThan
    a owl:ObjectProperty ;
    rdfs:comment "Indicates that the subject scale of measurement is more specific than (i.e. a special case of) the object scale of measurement."@en ;
    rdfs:domain :ScaleOfMeasurement ;
    rdfs:label "More specific than..."@en ;
    rdfs:range :ScaleOfMeasurement .

:Nominal
    a :ScaleOfMeasurementForCategoricalData, owl:NamedIndividual ;
    rdfs:comment "Scale of measurement for categorical data"@en ;
    rdfs:label "Nominal"@en .

:Ordinal
    a :ScaleOfMeasurementForCategoricalData, owl:NamedIndividual ;
    rdfs:comment "Scale of measurement for categorical data"@en ;
    rdfs:label "Ordinal"@en ;
    :moreSpecificThan :Nominal.

:Interval
    a :ScaleOfMeasurementForQuantitativeData, owl:NamedIndividual ;
    rdfs:comment "Scale of measurement for quantitative data"@en ;
    rdfs:label "Interval"@en .

:Ratio
    a :ScaleOfMeasurementForQuantitativeData, owl:NamedIndividual ;
    rdfs:comment "Scale of measurement for quantitative data"@en ;
    rdfs:label "Ratio"@en ;
    :moreSpecificThan :Interval.


:Angular
    a :ScaleOfMeasurementForQuantitativeData, owl:NamedIndividual ;
    rdfs:comment "Scale of measurement for angular data"@en ;
    rdfs:label "Angular"@en .

:GeographicLatitude
    a :ScaleOfMeasurementForQuantitativeData, owl:NamedIndividual ;
    rdfs:comment "Scale of measurement for geographic latitude"@en ;
    rdfs:label "Geographic Latitude"@en ;
    :moreSpecificThan :Angular.

:GeographicLongitude
    a :ScaleOfMeasurementForQuantitativeData, owl:NamedIndividual ;
    rdfs:comment "Scale of measurement for geographic longitude"@en ;
    rdfs:label "Geographic Longitude"@en ;
    :moreSpecificThan :Angular.
